address jon & rob's comment, move inv out, inv wip

Filesys/FileSystem.s.dfy
@@ -1,9 +1,7 @@
 // Copyright 2018-2021 VMware, Inc., Microsoft Inc., Carnegie Mellon University, ETH Zurich, and University of Washington
 // SPDX-License-Identifier: BSD-2-Clause
 
-
 include "FSTypes.s.dfy"
-include "../lib/Lang/System/SeqComparison.s.dfy"
 
 /*
  * This file system doesn't specify any permission checking or path cleanup: relying on shim/vfs to do so.
@@ -14,66 +12,57 @@ module FileSystem {
   import opened FSTypes
   import opened PathSpec
   import opened Options
-  import SeqComparison
 
-  type MetaView = imap<int, MetaData>
-  type DataView = imap<int, Data> 
+  type MetaView = imap<ID, MetaData>
+  type DataView = imap<ID, Data> 
 
   datatype FileSys = FileSys(path_map: PathMap, meta_map: MetaView, data_map: DataView)
 
   // jonh: This file would get 5.5% shorter if we replace WF with a subset type :)
+  // jialin: we don't have an easy function method to initialize these imaps for the witness
+  //   I saw splinter's interp.s example to bypass the compilation complaints but not sure if that's
+  //   the standard/style we want to go with, so just going to leave this predicate here for now
   predicate WF(fs: FileSys)
   {
-    && PathComplete(fs.path_map)
+    && PathMapComplete(fs.path_map)
     && (forall id :: id in fs.meta_map && id in fs.data_map)
   }
 
-  // robj: How about PathExists?
-  predicate ValidPath(fs: FileSys, path: Path)
+  predicate PathExists(fs: FileSys, path: Path)
   requires WF(fs)
   {
-    && fs.path_map[path] != DefaultId
+    && fs.path_map[path].ID?
     && fs.meta_map[fs.path_map[path]].MetaData?
   }
 
   predicate Init(fs: FileSys)
   {
     && fs.path_map == InitPathMap()
-    && fs.meta_map == (imap id :: if id == RootId then InitRootMetaData() else EmptyMetaData)
+    && fs.meta_map == (imap id :: if id == RootID then InitRootMetaData() else EmptyMetaData)
     && fs.data_map == (imap id :: EmptyData())
   }
 
   /// Inv conditions
 
-  function AliasPaths(fs: FileSys, id: int) : (aliases: iset<Path>)
+  function AliasPaths(fs: FileSys, id: ID) : (aliases: iset<Path>)
   requires WF(fs)
-  ensures forall path | path !in aliases :: fs.path_map[path] != id
- // jonh suggest strethening to:
-  ensures forall path | path in aliases <==> fs.path_map[path] == id
-  // although it's not opaque, so you can delete all the ensures and dafny can just derive
-  // both.
+  ensures forall path :: path in aliases <==> fs.path_map[path] == id
   {
     iset path | fs.path_map[path] == id
   }
 
-  // robj: why require both the id and the path?
-  predicate NoAlias(fs: FileSys, id: int, path: Path)
+  predicate NoAlias(fs: FileSys, path: Path)
   requires WF(fs)
-  requires fs.path_map[path] == id
   {
-    && AliasPaths(fs, id) == iset{path}
+    && AliasPaths(fs, fs.path_map[path]) == iset{path}
   }
 
-  // robj: How about DirImpliesHasNoAlias?
-  // jonh: notes how hard you're working to encode hardlinks, which Zeus gave to mortals
-  // for a weekend prank.
-  predicate DirHasNoAlias(fs: FileSys, path: Path)
+  predicate DirImpliesHasNoAlias(fs: FileSys, path: Path)
   requires WF(fs)
-  requires ValidPath(fs, path)
+  requires PathExists(fs, path)
   {
     var id := fs.path_map[path];
-    var m := fs.meta_map[id];
-    && (m.ftype.Directory? ==> NoAlias(fs, id, path))
+    && (fs.meta_map[id].ftype.Directory? ==> NoAlias(fs, path))
   }
 
   predicate ParentDirIsDir(fs: FileSys, path: Path)
@@ -81,25 +70,21 @@ module FileSystem {
   {
     var parent_dir := GetParentDir(path);
     var parent_id := fs.path_map[parent_dir];
-    && ValidPath(fs, parent_dir)
+    && PathExists(fs, parent_dir)
     && fs.meta_map[parent_id].ftype.Directory?
   }
 
-  // robj: Can we kill the middle line of this predicate?  It seems
-  // like it's implied by the first line and the last lemma in
-  // PathSpec.s.dfy.
   predicate ValidNewPath(fs: FileSys, path: Path)
   requires WF(fs)
   {
     && ParentDirIsDir(fs, path)
-    && IsDirEntry(GetParentDir(path), path)
-    && fs.path_map[path] == DefaultId
+    && fs.path_map[path].Nonexistent?
   }
 
-  predicate ValidNewId(fs: FileSys, id: int)
+  predicate ValidNewId(fs: FileSys, id: ID)
   requires WF(fs)
   {
-    && id != DefaultId
+    && id.ID?
     && AliasPaths(fs, id) == iset{}
   }
 
@@ -108,7 +93,7 @@ module FileSystem {
   predicate GetAttr(fs: FileSys, fs':FileSys, path: Path, attr: MetaData)
   {
     && WF(fs)
-    && ValidPath(fs, path)
+    && PathExists(fs, path)
     && fs' == fs
     && attr == fs.meta_map[fs.path_map[path]]
   }
@@ -116,15 +101,26 @@ module FileSystem {
   predicate ReadLink(fs: FileSys, fs':FileSys, path: Path, link_path: Path)
   {
     && WF(fs)
-    && ValidPath(fs, path)
+    && PathExists(fs, path)
     && fs' == fs
     && fs.meta_map[fs.path_map[path]].ftype.SymLink?
     && link_path == fs.meta_map[fs.path_map[path]].ftype.source
   }
 
+  function UpdateParentTime(fs: FileSys, id: ID, time: Time) : MetaData
+  requires WF(fs)
+  {
+    var m := fs.meta_map[id];
+    if m.MetaData? then (
+      MetaDataUpdateTime(m, m.atime, time, time)
+    ) else (
+      m
+    )
+  }
+
   // robj: Need to update mtime of parent dir (and same for other
-  // directory mutations, e.g. symlink, delete, link, etc)
-  predicate Create(fs: FileSys, fs':FileSys, path: Path, id: int, m: MetaData)
+  // directory mutations, e.g. delete, link, etc)
+  predicate Create(fs: FileSys, fs':FileSys, path: Path, id: ID, m: MetaData)
   {
     && WF(fs)
     && WF(fs')
@@ -132,11 +128,12 @@ module FileSystem {
     && ValidNewMetaData(m, path)
     && ValidNewId(fs, id)
     // Entry Not Present
-    && fs.meta_map[id].EmptyMetaData?
-    && fs.data_map[id] == EmptyData()
+    // && fs.meta_map[id].EmptyMetaData?
+    // && fs.data_map[id] == EmptyData() // jialin: might be able to derive these from inv
     // Updated maps
+    && var parent_id := fs.path_map[GetParentDir(path)];
     && fs'.path_map == fs.path_map[path := id]
-    && fs'.meta_map == fs.meta_map[id := m]
+    && fs'.meta_map == fs.meta_map[id := m][parent_id := UpdateParentTime(fs, parent_id, m.mtime)]
     && fs'.data_map == fs.data_map
   }
 
@@ -148,21 +145,18 @@ module FileSystem {
 
   function MetaDataDelete(fs: FileSys, path: Path, ctime: Time): MetaData
   requires WF(fs)
-  requires ValidPath(fs, path)
   {
     var id := fs.path_map[path];
-
-    if NoAlias(fs, id, path)
+    if id.Nonexistent? || fs.meta_map[id].EmptyMetaData? || NoAlias(fs, path)
     then EmptyMetaData
     else MetaDataUpdateCTime(fs.meta_map[id], ctime)
   }
 
   function DataDelete(fs: FileSys, path: Path): Data
   requires WF(fs)
-  requires ValidPath(fs, path)
   {
     var id := fs.path_map[path];
-    if NoAlias(fs, id, path)
+    if id.Nonexistent? || NoAlias(fs, path)
     then EmptyData()
     else fs.data_map[id]
   }
@@ -172,114 +166,63 @@ module FileSystem {
     && WF(fs)
     && WF(fs')
     && path != RootDir
-    && ValidPath(fs, path)
+    && PathExists(fs, path)
     && var id := fs.path_map[path];
     && (fs.meta_map[id].ftype.Directory? ==> IsEmptyDir(fs.path_map, path))
     // maps after delete
-    && fs'.path_map == fs.path_map[path := DefaultId]
-    && fs'.meta_map == fs.meta_map[id := MetaDataDelete(fs, path, ctime)]
+    && var parent_id := fs.path_map[GetParentDir(path)];
+    && fs'.path_map == fs.path_map[path := Nonexistent]
+    && fs'.meta_map == fs.meta_map[id := MetaDataDelete(fs, path, ctime)][parent_id := UpdateParentTime(fs, parent_id, ctime)]
     && fs'.data_map == fs.data_map[id := DataDelete(fs, path)]
   }
 
-  // robj: This seems like a special case of Create
-  predicate SymLink(fs: FileSys, fs':FileSys, source: Path, dest: Path, id: int, m: MetaData)
-  {
-    && WF(fs)
-    && WF(fs')
-    && ValidNewPath(fs, dest) // source doesn't need to be valid
-    && ValidNewMetaData(m, dest)
-    && m.ftype == FileType.SymLink(source)
-    && ValidNewId(fs, id)
-    && fs.meta_map[id] == EmptyMetaData
-    && fs.data_map[id] == EmptyData()
-    // updated maps
-    && fs'.path_map == fs.path_map[dest := id]
-    && fs'.meta_map == fs.meta_map[id := m]
-    && fs'.data_map == fs.data_map
-  }
-
-  function PathMapRenameDir(fs: FileSys, src: Path, dst: Path): (path_map: PathMap)
+  function PathMapRename(fs: FileSys, src: Path, dst: Path): (path_map: PathMap)
   requires WF(fs)
-  ensures PathComplete(path_map)
+  ensures PathMapComplete(path_map)
   ensures 
-    forall p | p != src && !InDir(src, p) && p != dst && !InDir(dst, p)
+    forall p | p != src && !BeneathDir(src, p) && p != dst && !BeneathDir(dst, p)
       :: path_map[p] == fs.path_map[p]
   {
     imap path :: 
       // remove source paths
-      if path == src || InDir(src, path) then DefaultId
+      if path == src || BeneathDir(src, path) then Nonexistent
       // redirect renamed paths to point to the same ids as source
-      else if path == dst || InDir(dst, path) then fs.path_map[src + path[|dst|..]]
+      else if path == dst || BeneathDir(dst, path) then fs.path_map[src + path[|dst|..]]
       // everything else remains the same
       else fs.path_map[path]
   }
 
-  // robj: Can we unify the dir and non-dir cases?  If the only
-  // difference is renaming all the entries below the dir, then for
-  // non-dirs, that should be a no-op.
-  // jonh: ditto -- yeah, I think it's worth trying; should be tighter.
-  predicate RenameDir(fs: FileSys, fs':FileSys, src: Path, dst: Path, ctime: Time)
-  requires WF(fs)
-  requires WF(fs')
-  requires ValidPath(fs, src)
-  requires ValidPath(fs, dst) || ValidNewPath(fs, dst)
-  {
-    var src_id := fs.path_map[src];
-    var dst_id := fs.path_map[dst];
-    var src_m := fs.meta_map[src_id];
-    var src_m' := MetaDataUpdateCTime(src_m, ctime);
-    // NOTE(Jialin): temporary path restriction
-    && |src| > 1
-    && |dst| > 1
-    // end of temporary path restrictions
-    && src_m.ftype.Directory?
-    && (ValidPath(fs, dst) ==>
-      && fs.meta_map[fs.path_map[dst]].ftype.Directory?
-      && IsEmptyDir(fs.path_map, dst))
-    // updated maps
-    && fs'.path_map == PathMapRenameDir(fs, src, dst)
-    && fs'.meta_map == (
-      if ValidPath(fs, dst)
-      // robj: are src and dst reversed here?
-      then fs.meta_map[src_id := src_m'][dst_id := EmptyMetaData]
-      else fs.meta_map[src_id := src_m'])
-    && fs'.data_map == fs.data_map
-  }
-
-  predicate RenameNonDir(fs: FileSys, fs':FileSys, src: Path, dst: Path, ctime: Time)
-  requires WF(fs)
-  requires WF(fs')
-  requires ValidPath(fs, src)
-  requires ValidPath(fs, dst) || ValidNewPath(fs, dst)
-  {
-    var src_id := fs.path_map[src];
-    var dst_id := fs.path_map[dst];
-    var src_m := fs.meta_map[src_id];
-    var src_m' := MetaDataUpdateCTime(src_m, ctime);
-    && !src_m.ftype.Directory? // file, symlink, dev file, fifo, socket
-    // updated maps
-    && fs'.path_map == fs.path_map[dst := src_id][src := DefaultId]
-    && (ValidPath(fs, dst) ==> 
-      && src_id != dst_id
-      && !fs.meta_map[dst_id].ftype.Directory?
-      && fs'.meta_map == fs.meta_map[src_id := src_m'][dst_id := MetaDataDelete(fs, dst, ctime)]
-      && fs'.data_map == fs.data_map[dst_id := DataDelete(fs, dst)])
-    && (!ValidPath(fs, dst) ==>
-      && fs'.meta_map == fs.meta_map[src_id := src_m']
-      && fs'.data_map == fs.data_map)
-  }
-
-  // rename is a map because we allow directory
   predicate Rename(fs: FileSys, fs':FileSys, src: Path, dst: Path, ctime: Time)
   {
     && WF(fs)
     && WF(fs')
-    && ValidPath(fs, src)
-    && !InDir(dst, src)
-    && (ValidPath(fs, dst) || ValidNewPath(fs, dst))
-    && var src_m := fs.meta_map[fs.path_map[src]];
-    && (src_m.ftype.Directory? ==> RenameDir(fs, fs', src, dst, ctime))
-    && (!src_m.ftype.Directory? ==> RenameNonDir(fs, fs', src, dst, ctime))
+    && PathExists(fs, src)
+    && !BeneathDir(dst, src)
+    && (PathExists(fs, dst) || ValidNewPath(fs, dst))
+
+    && var src_id := fs.path_map[src];
+    && var dst_id := fs.path_map[dst];
+    && var src_m := fs.meta_map[src_id];
+    && (PathExists(fs, dst) ==> 
+      && var dst_m := fs.meta_map[dst_id];
+      && (src_m.ftype.Directory? <==> dst_m.ftype.Directory?)
+      && (dst_m.ftype.Directory? ==> IsEmptyDir(fs.path_map, dst))
+    )
+
+    && var sparent_id := fs.path_map[GetParentDir(src)];
+    && var dparent_id := fs.path_map[GetParentDir(dst)];
+    && var src_m' := MetaDataUpdateCTime(src_m, ctime);
+    && fs'.path_map == PathMapRename(fs, src, dst)
+    // robj: are src and dst reversed here?
+    // jialin: src changes to dst in fs', but dst still points to the src_id
+    //  so we update src_id to src_m', and delete anything that might be pointed to dst
+    //  to show any old content is overwritten   
+    && fs'.meta_map == 
+          fs.meta_map[src_id := src_m']
+                     [dst_id := MetaDataDelete(fs, dst, ctime)]
+                     [sparent_id := UpdateParentTime(fs, sparent_id, ctime)]
+                     [dparent_id := UpdateParentTime(fs, dparent_id, ctime)]
+    && fs'.data_map == fs.data_map[dst_id := DataDelete(fs, dst)]
   }
 
   predicate Link(fs: FileSys, fs':FileSys, source: Path, dest: Path, ctime: Time)
@@ -288,14 +231,15 @@ module FileSystem {
     && WF(fs')
     // NOTE: won't work for hardlink other filesystem files
     // robj: Hard-links can't cross file systems, so not a problem.
-    && ValidPath(fs, source)
+    && PathExists(fs, source)
     && ValidNewPath(fs, dest)
     && var id := fs.path_map[source];
     && var m := fs.meta_map[id];
     && !m.ftype.Directory?  // disallow directory hardlinks
     // updated maps
+    && var dparent_id := fs.path_map[GetParentDir(dest)];
     && fs'.path_map == fs.path_map[dest := id]
-    && fs'.meta_map == fs.meta_map[id := MetaDataUpdateCTime(m, ctime)]
+    && fs'.meta_map == fs.meta_map[id := MetaDataUpdateCTime(m, ctime)][dparent_id := UpdateParentTime(fs, dparent_id, ctime)]
     && fs'.data_map == fs.data_map
   }
 
@@ -310,7 +254,7 @@ module FileSystem {
   {
     && WF(fs)
     && WF(fs')
-    && ValidPath(fs, path)
+    && PathExists(fs, path)
     && var id := fs.path_map[path];
     && fs'.path_map == fs.path_map
     && fs'.meta_map == fs.meta_map[id := MetaDataChangeAttr(fs.meta_map[id], perm, uid, gid, ctime)]
@@ -327,14 +271,6 @@ module FileSystem {
   function ZeroData(size: nat) : (d: Data) { seq(size, i => 0) }
   // don't need any requires or ensures!
 
-  function ZeroData(size: int) : (d: Data)
-  requires size >= 0
-  ensures size == |d|
-  ensures forall i | 0 <= i < |d| :: d[i] == 0
-  {
-    if size == 0 then [] else ZeroData(size-1) + [0]
-  }
-
   function DataTruncate(d: Data, size: int): (d': Data)
   requires 0 <= size
   ensures |d'| == size
@@ -347,11 +283,10 @@ module FileSystem {
     && WF(fs)
     && WF(fs')
     && 0 <= size
-    && ValidPath(fs, path)
+    && PathExists(fs, path)
     && var id := fs.path_map[path];
     && var m := fs.meta_map[id];
     && m.ftype.File?
-    && size != |fs.data_map[id]| // robj: Need this?
     // updated maps
     && fs'.path_map == fs.path_map
     && fs'.meta_map == fs.meta_map[id := MetaDataUpdateTime(m, m.atime, time, time)]
@@ -362,7 +297,7 @@ module FileSystem {
   {
     && WF(fs)
     && fs' == fs
-    && ValidPath(fs, path)
+    && PathExists(fs, path)
     && var id := fs.path_map[path];
     && fs.meta_map[id].ftype.File?
     && 0 <= offset <= offset+size <= |fs.data_map[id]|
@@ -382,7 +317,7 @@ module FileSystem {
   {
     && WF(fs)
     && WF(fs')
-    && ValidPath(fs, path)
+    && PathExists(fs, path)
     && |data| == size
     && var id := fs.path_map[path];
     && var m := fs.meta_map[id];
@@ -398,7 +333,7 @@ module FileSystem {
   {
     && WF(fs)
     && WF(fs')
-    && ValidPath(fs, path)
+    && PathExists(fs, path)
     && var id := fs.path_map[path];
     && fs'.path_map == fs.path_map
     && fs'.meta_map == fs.meta_map[id := MetaDataUpdateTime(fs.meta_map[id], atime, mtime, ctime)]
@@ -408,33 +343,38 @@ module FileSystem {
   predicate ValidDirEntry(fs: FileSys, de: DirEntry)
   requires WF(fs)
   {
-    && ValidPath(fs, de.path) // valid path
+    && PathExists(fs, de.path)
     && de.id == fs.path_map[de.path]
     && de.ftype == fs.meta_map[de.id].ftype
   }
 
   // robj: What about done?
   // robj: Should we requires that results are all >= start in sort order?
+  // jialin: just updated line 404-406
   predicate ReadDir(fs: FileSys, fs':FileSys, dir: Path, start: Option<Path>, results: seq<DirEntry>, done: bool)
   {
     && WF(fs)
     && fs' == fs
-    && ValidPath(fs, dir)
+    && PathExists(fs, dir)
     && fs.meta_map[fs.path_map[dir]].ftype.Directory?
-    && (start.Some? ==> InDir(dir, start.value)) // robj: Should this be IsDirEntry?  I guess InDir would work, but a little odd
-    // results consistent with filesys content
-    && (forall i | 0 <= i < |results| :: ValidDirEntry(fs, results[i]))
+    && (start.Some? ==> IsDirEntry(dir, start.value))
     // results actually belong to this directory
     && (forall i | 0 <= i < |results| :: IsDirEntry(dir, results[i].path))
-    // results are strictly sorted
-    && (forall i, j | 0 <= i < j < |results| :: SeqComparison.lt(results[i].path, results[j].path))
+    // results consistent with filesys content
+    && (forall i | 0 <= i < |results| :: ValidDirEntry(fs, results[i]))
+    // results are strictly sorted, >= start
+    && (start.Some? && |results| > 0 ==> DirEntryLte(start.value, results[0].path))
+    && (forall i, j | 0 <= i < j < |results| :: 
+          && DirEntryLte(results[i].path, results[j].path)
+          && results[i] != results[j])
     // results don't skip over any valid entry
     && (forall path |
         && IsDirEntry(dir, path)
-        && ValidPath(fs, path)
-        && (start.Some? ==> SeqComparison.lte(path, start.value))
-        && (!done && |results| > 0 ==> SeqComparison.lt(results[|results|-1].path, path))
-        :: (exists i :: 0 <= i < |results| && results[i].path == path))
+        && PathExists(fs, path)
+        && (start.Some? ==> DirEntryLte(start.value, path))
+        && (done ==> (exists i :: 0 <= i < |results| && results[i].path == path))
+        && (!done && |results| > 0 ==> DirEntryLte(path, results[|results|-1].path))
+          :: (exists i :: 0 <= i < |results| && results[i].path == path))
   }
 
   predicate Stutter(fs: FileSys, fs': FileSys)
@@ -446,9 +386,8 @@ module FileSystem {
   datatype Step =
     | GetAttrStep(path: Path, attr: MetaData)
     | ReadLinkStep(path: Path, link_path: Path)
-    | CreateStep(path: Path, id: int, m: MetaData) // mknod and mkdir
+    | CreateStep(path: Path, id: ID, m: MetaData) // mknod, mkdir, symlink
     | DeleteStep(path: Path, ctime: Time) // unlink and rmdir
-    | SymLinkStep(source: Path, dest: Path, id: int, m: MetaData)
     | RenameStep(source: Path, dest: Path, ctime: Time)
     | LinkStep(source: Path, dest: Path, ctime: Time)
     | ChangeAttrStep(path: Path, perm: int, uid: int, gid: int, ctime: Time) // chmod + chown
@@ -466,7 +405,6 @@ module FileSystem {
       case ReadLinkStep(path, link_path) => ReadLink(fs, fs', path, link_path)
       case CreateStep(path, id, m) => Create(fs, fs', path, id, m)
       case DeleteStep(path, ctime) => Delete(fs, fs', path, ctime)
-      case SymLinkStep(source, dest, id, m) => SymLink(fs, fs', source, dest, id, m)
       case RenameStep(source, dest, ctime) => Rename(fs, fs', source, dest, ctime)
       case LinkStep(source, dest, ctime) => Link(fs, fs', source, dest, ctime)
       case ChangeAttrStep(path, perm, uid, gid, ctime) => ChangeAttr(fs, fs', path, perm, uid, gid, ctime)
@@ -482,262 +420,5 @@ module FileSystem {
   predicate Next(fs: FileSys, fs': FileSys)
   {
     exists step :: NextStep(fs, fs', step)
-  }
-
-  // robj: I think all this stuff from here on down should be moved to a .i.dfy file
-
-  predicate Inv(fs: FileSys)
-  {
-    && WF(fs)
-    // DefaultId is never occupied
-    && fs.meta_map[DefaultId].EmptyMetaData?
-    && fs.data_map[DefaultId] == EmptyData()
-    // Path map internal invariant :: all valid paths must be greater than 0
-    && (forall path | ValidPath(fs, path) :: |path| > 0) // all valid path must 
-    // Metadata map internal consistency: nlink consitency and directory has no hardlinks
-    && (forall path | ValidPath(fs, path) :: DirHasNoAlias(fs, path))
-    // Path and meta map consistency: directory structure is connected
-    && (forall path | ValidPath(fs, path) && path != RootDir :: ParentDirIsDir(fs, path))
-  }
-
-  lemma InitImpliesInv(fs: FileSys)
-  requires Init(fs)
-  ensures Inv(fs)
-  {
-  }
-
-  // TODO: add ui op
-  lemma NextPreservesInv(fs: FileSys, fs': FileSys)
-  requires Inv(fs)
-  requires Next(fs, fs')
-  ensures Inv(fs')
-  {
-    var step :| NextStep(fs, fs', step);
-    NextStepPreservesInv(fs, fs', step);
-  }
-
-  lemma NextStepPreservesInv(fs: FileSys, fs': FileSys, step: Step)
-  requires Inv(fs)
-  requires NextStep(fs, fs', step)
-  ensures Inv(fs')
-  {
-    match step {
-      case DeleteStep(path, ctime) => DeletePreservesInv(fs, fs', path, ctime);
-      case RenameStep(source, dest, ctime) => RenamePreservesInv(fs, fs', source, dest, ctime);
-      case LinkStep(source, dest, ctime) => LinkPreservesInv(fs, fs', source, dest, ctime); 
-      case _ => {
-        if step.CreateStep? || step.SymLinkStep? || step.ChangeAttrStep? 
-        || step.TruncateStep? || step.WriteStep? || step.UpdateTimeStep? {
-          SimpleStepPreservesInv(fs, fs', step);
-        }
-      }
-    }
-  }
-
-  /// Invariant proofs
-
-  lemma SameAliases(fs: FileSys, fs': FileSys, changedPaths: iset<Path>, changedIds: iset<int>)
-  requires Inv(fs)
-  requires WF(fs')
-  requires forall p | p in changedPaths :: fs.path_map[p] in changedIds || fs.path_map[p] == DefaultId
-  requires forall p | p in changedPaths :: fs'.path_map[p] in changedIds || fs'.path_map[p] == DefaultId
-  requires forall p | p !in changedPaths :: fs'.path_map[p] == fs.path_map[p]
-  requires forall p | p !in changedPaths :: fs'.path_map[p] !in changedIds
-  ensures forall p | ValidPath(fs, p) && ValidPath(fs', p) && p !in changedPaths ::
-    AliasPaths(fs, fs.path_map[p]) == AliasPaths(fs', fs'.path_map[p])
-  {
-  }
-
-  lemma DeletePreservesInv(fs: FileSys, fs': FileSys, path: Path, ctime: Time)
-  requires Inv(fs)
-  requires Delete(fs, fs', path, ctime)
-  ensures Inv(fs')
-  {
-    forall p | ValidPath(fs', p)
-    ensures DirHasNoAlias(fs', p)
-    ensures p != RootDir ==> ParentDirIsDir(fs', p)
-    {
-      assert DirHasNoAlias(fs, p); // observe
-      assert p != RootDir ==> ParentDirIsDir(fs, p); // observe
-  
-      var id := fs.path_map[path];
-      if fs'.path_map[p] != id {
-        SameAliases(fs, fs', AliasPaths(fs, id), iset{id});
-      }
-    }
-
-    assert Inv(fs');
-  }
-
-  lemma RenameNonDirPreservesInv(fs: FileSys, fs': FileSys, src: Path, dst: Path, ctime: Time)
-  requires Inv(fs)
-  requires Rename(fs, fs', src, dst, ctime)
-  requires RenameNonDir(fs, fs', src, dst, ctime)
-  ensures Inv(fs')
-  {
-    assert fs'.meta_map[DefaultId].EmptyMetaData?; // observe
-
-    forall p | ValidPath(fs', p)
-    ensures DirHasNoAlias(fs', p)
-    ensures p != RootDir ==> ParentDirIsDir(fs', p)
-    {
-      var src_id := fs.path_map[src];
-      var dst_id := fs.path_map[dst];
-
-      if fs'.path_map[p] != src_id && fs'.path_map[p] != dst_id {
-        var changedIds := if ValidPath(fs, dst) then iset{src_id, dst_id} else iset{src_id};
-        var changedPaths := iset path | fs.path_map[path] in changedIds || fs'.path_map[path] in changedIds;
-        SameAliases(fs, fs', changedPaths, changedIds);
-        assert DirHasNoAlias(fs, p);
-      }
-      assert DirHasNoAlias(fs', p);
-
-      if p != RootDir {
-        assert ParentDirIsDir(fs, p); // observe
-        assert ParentDirIsDir(fs', p);
-      }
-    }
-    assert Inv(fs');
-  }
-
-  lemma RenamedPathsRemainDifferent(src: Path, dst: Path, p1: Path, p2: Path)
-  requires p1 != p2
-  requires p1 == dst || InDir(dst, p1)
-  requires p2 == dst || InDir(dst, p2)
-  ensures src + p1[|dst|..] != src + p2[|dst|..]
-  {
-    if InDir(dst, p1) && InDir(dst, p2) {
-      assert p1[|dst|..] != p2[|dst|..];
-
-      var p1' := src + p1[|dst|..];
-      var p2' := src + p2[|dst|..];
-
-      assert p1'[..|src|] == p2'[..|src|];
-    }
-  }
-
-  lemma RenameDirPreservesInv(fs: FileSys, fs': FileSys, src: Path, dst: Path, ctime: Time)
-  requires Inv(fs)
-  requires Rename(fs, fs', src, dst, ctime)
-  requires RenameDir(fs, fs', src, dst, ctime)
-  ensures Inv(fs')
-  {
-    forall p | ValidPath(fs', p)
-    ensures DirHasNoAlias(fs', p)
-    ensures p != RootDir ==> ParentDirIsDir(fs', p)
-    {
-      assert |p| > 0;
-      if p != RootDir {
-        var parent_dir := GetParentDir(p);
-        var parent_id := fs.path_map[parent_dir];
-
-        if p == dst {
-        } else if InDir(dst, p) {
-          var srcpath := src + p[|dst|..];
-          var srcparent_dir := GetParentDir(srcpath);
-          assert ParentDirIsDir(fs, srcpath);
-          assert parent_dir == dst || InDir(dst, parent_dir); // observe
-          assert src + parent_dir[|dst|..] == srcparent_dir; // observe
-        } else {
-          assert ValidPath(fs, p);
-          assert ParentDirIsDir(fs, p); // observe
-          assert fs.path_map[parent_dir] == fs'.path_map[parent_dir];
-        }
-        assert ParentDirIsDir(fs', p);
-      }
-
-      var id := fs'.path_map[p];
-      var m := fs'.meta_map[id];
-      var aliases := AliasPaths(fs', id);
-
-      if (exists path | path in aliases :: path == dst || InDir(dst, path)) {
-        // this covers cases for dst prefixes and old src's aliases
-        if m.ftype.Directory? && !NoAlias(fs', id, p) {
-          var path :| path in aliases && (path == dst || InDir(dst, path));
-          var aliaspath :| aliaspath in aliases && aliaspath != path;
-          assert path != aliaspath;
-
-          var srcpath := src + path[|dst|..];
-          assert id == fs.path_map[srcpath];
-          assert DirHasNoAlias(fs, srcpath); // observe
-
-          if aliaspath == dst || InDir(dst, aliaspath) {
-            var srcalias := src + aliaspath[|dst|..];
-            assert fs.path_map[srcalias] == fs'.path_map[aliaspath];
-            RenamedPathsRemainDifferent(src, dst, path, aliaspath);
-            assert srcalias != srcpath;
-            assert false;
-          } else {
-            assert fs.path_map[aliaspath] == fs'.path_map[aliaspath]; 
-            assert false;
-          }
-        }
-      } else {
-        assert DirHasNoAlias(fs, p); // observe
-        assert DirHasNoAlias(fs', p);
-      }
-    }
-  
-    assert Inv(fs');
-  }
-
-  lemma RenamePreservesInv(fs: FileSys, fs': FileSys, source: Path, dest: Path, ctime: Time)
-  requires Inv(fs)
-  requires Rename(fs, fs', source, dest, ctime)
-  ensures Inv(fs')
-  {
-    var m := fs.meta_map[fs.path_map[source]];
-    if m.ftype.Directory? {
-      RenameDirPreservesInv(fs, fs', source, dest, ctime);
-    } else {
-      RenameNonDirPreservesInv(fs, fs', source, dest, ctime);
-    }
-  }
-
-  lemma LinkPreservesInv(fs: FileSys, fs': FileSys, source: Path, dest: Path, ctime: Time)
-  requires Inv(fs)
-  requires Link(fs, fs', source, dest, ctime)
-  ensures Inv(fs')
-  {
-    forall p | ValidPath(fs', p)
-    ensures DirHasNoAlias(fs', p)
-    ensures p != RootDir ==> ParentDirIsDir(fs', p)
-    {
-      assert p != dest ==> DirHasNoAlias(fs, p); // observe
-      assert p != RootDir ==> ParentDirIsDir(fs, p); // observe
-
-      var id := fs.path_map[source];
-      if fs'.path_map[p] != id {
-        SameAliases(fs, fs', AliasPaths(fs', id), iset{id});
-      }
-    }
-
-    assert Inv(fs');
-  }
-
-  lemma SimpleStepPreservesInv(fs: FileSys, fs': FileSys, step: Step)
-  requires Inv(fs)
-  requires NextStep(fs, fs', step)
-  requires step.CreateStep? || step.SymLinkStep? || step.ChangeAttrStep?
-        || step.TruncateStep? || step.WriteStep? || step.UpdateTimeStep?
-  ensures Inv(fs')
-  {
-    var path := if step.SymLinkStep? then step.dest else step.path;
-
-    forall p | ValidPath(fs', p)
-    ensures DirHasNoAlias(fs', p)
-    ensures p != RootDir ==> ParentDirIsDir(fs', p)
-    {
-      if p != path {
-        assert ValidPath(fs, p); // observe
-        assert DirHasNoAlias(fs, p); // observe
-
-        if step.SymLinkStep? || step.CreateStep? {
-          SameAliases(fs, fs', iset{path}, iset{fs'.path_map[path]});
-        }
-      }
-    }
-
-    assert Inv(fs');
   }
 }
