Filesys/FileSystemInv.i.dfy
@@ -1,0 +1,267 @@
+// Copyright 2018-2021 VMware, Inc., Microsoft Inc., Carnegie Mellon University, ETH Zurich, and University of Washington
+// SPDX-License-Identifier: BSD-2-Clause
+
+include "FileSystem.s.dfy"
+
+module FileSystemInv {
+  import opened FileSystem
+  import opened FSTypes
+  import opened PathSpec
+
+//   predicate Inv(fs: FileSys)
+//   {
+//     && WF(fs)
+//     // DefaultId is never occupied
+//     && fs.meta_map[DefaultId].EmptyMetaData?
+//     && fs.data_map[DefaultId] == EmptyData()
+//     // Path map internal invariant :: all valid paths must be greater than 0
+//     && (forall path | PathExists(fs, path) :: |path| > 0) // all valid path must 
+//     // Metadata map internal consistency: nlink consitency and directory has no hardlinks
+//     && (forall path | PathExists(fs, path) :: DirImpliesHasNoAlias(fs, path))
+//     // Path and meta map consistency: directory structure is connected
+//     && (forall path | PathExists(fs, path) && path != RootDir :: ParentDirIsDir(fs, path))
+//   }
+
+//   lemma InitImpliesInv(fs: FileSys)
+//   requires Init(fs)
+//   ensures Inv(fs)
+//   {
+//   }
+
+//   // TODO: add ui op
+//   lemma NextPreservesInv(fs: FileSys, fs': FileSys)
+//   requires Inv(fs)
+//   requires Next(fs, fs')
+//   ensures Inv(fs')
+//   {
+//     var step :| NextStep(fs, fs', step);
+//     NextStepPreservesInv(fs, fs', step);
+//   }
+
+//   lemma NextStepPreservesInv(fs: FileSys, fs': FileSys, step: Step)
+//   requires Inv(fs)
+//   requires NextStep(fs, fs', step)
+//   ensures Inv(fs')
+//   {
+//     match step {
+//       case DeleteStep(path, ctime) => DeletePreservesInv(fs, fs', path, ctime);
+//       case RenameStep(source, dest, ctime) => RenamePreservesInv(fs, fs', source, dest, ctime);
+//       case LinkStep(source, dest, ctime) => LinkPreservesInv(fs, fs', source, dest, ctime); 
+//       case _ => {
+//         if step.CreateStep? || step.SymLinkStep? || step.ChangeAttrStep? 
+//         || step.TruncateStep? || step.WriteStep? || step.UpdateTimeStep? {
+//           SimpleStepPreservesInv(fs, fs', step);
+//         }
+//       }
+//     }
+//   }
+
+//   /// Invariant proofs
+
+//   lemma SameAliases(fs: FileSys, fs': FileSys, changedPaths: iset<Path>, changedIds: iset<int>)
+//   requires Inv(fs)
+//   requires WF(fs')
+//   requires forall p | p in changedPaths :: fs.path_map[p] in changedIds || fs.path_map[p] == DefaultId
+//   requires forall p | p in changedPaths :: fs'.path_map[p] in changedIds || fs'.path_map[p] == DefaultId
+//   requires forall p | p !in changedPaths :: fs'.path_map[p] == fs.path_map[p]
+//   requires forall p | p !in changedPaths :: fs'.path_map[p] !in changedIds
+//   ensures forall p | PathExists(fs, p) && PathExists(fs', p) && p !in changedPaths ::
+//     AliasPaths(fs, fs.path_map[p]) == AliasPaths(fs', fs'.path_map[p])
+//   {
+//   }
+
+//   lemma DeletePreservesInv(fs: FileSys, fs': FileSys, path: Path, ctime: Time)
+//   requires Inv(fs)
+//   requires Delete(fs, fs', path, ctime)
+//   ensures Inv(fs')
+//   {
+//     assume false;
+//     forall p | PathExists(fs', p)
+//     ensures DirImpliesHasNoAlias(fs', p)
+//     ensures p != RootDir ==> ParentDirIsDir(fs', p)
+//     {
+//       assert DirImpliesHasNoAlias(fs, p); // observe
+//       assert p != RootDir ==> ParentDirIsDir(fs, p); // observe
+  
+//       var id := fs.path_map[path];
+//       if fs'.path_map[p] != id {
+//         SameAliases(fs, fs', AliasPaths(fs, id), iset{id});
+//       }
+//     }
+
+//     assert Inv(fs');
+//   }
+
+//   lemma RenameNonDirPreservesInv(fs: FileSys, fs': FileSys, src: Path, dst: Path, ctime: Time)
+//   requires Inv(fs)
+//   requires Rename(fs, fs', src, dst, ctime)
+//   requires RenameNonDir(fs, fs', src, dst, ctime)
+//   ensures Inv(fs')
+//   {
+//     assume false;
+//     assert fs'.meta_map[DefaultId].EmptyMetaData?; // observe
+
+//     forall p | PathExists(fs', p)
+//     ensures DirImpliesHasNoAlias(fs', p)
+//     ensures p != RootDir ==> ParentDirIsDir(fs', p)
+//     {
+//       var src_id := fs.path_map[src];
+//       var dst_id := fs.path_map[dst];
+
+//       if fs'.path_map[p] != src_id && fs'.path_map[p] != dst_id {
+//         var changedIds := if PathExists(fs, dst) then iset{src_id, dst_id} else iset{src_id};
+//         var changedPaths := iset path | fs.path_map[path] in changedIds || fs'.path_map[path] in changedIds;
+//         SameAliases(fs, fs', changedPaths, changedIds);
+//         assert DirImpliesHasNoAlias(fs, p);
+//       }
+//       assert DirImpliesHasNoAlias(fs', p);
+
+//       if p != RootDir {
+//         assert ParentDirIsDir(fs, p); // observe
+//         assert ParentDirIsDir(fs', p);
+//       }
+//     }
+//     assert Inv(fs');
+//   }
+
+//   lemma RenamedPathsRemainDifferent(src: Path, dst: Path, p1: Path, p2: Path)
+//   requires p1 != p2
+//   requires p1 == dst || InDir(dst, p1)
+//   requires p2 == dst || InDir(dst, p2)
+//   ensures src + p1[|dst|..] != src + p2[|dst|..]
+//   {
+//     if InDir(dst, p1) && InDir(dst, p2) {
+//       assert p1[|dst|..] != p2[|dst|..];
+
+//       var p1' := src + p1[|dst|..];
+//       var p2' := src + p2[|dst|..];
+
+//       assert p1'[..|src|] == p2'[..|src|];
+//     }
+//   }
+
+//   lemma RenameDirPreservesInv(fs: FileSys, fs': FileSys, src: Path, dst: Path, ctime: Time)
+//   requires Inv(fs)
+//   requires Rename(fs, fs', src, dst, ctime)
+//   requires RenameDir(fs, fs', src, dst, ctime)
+//   ensures Inv(fs')
+//   {
+//     forall p | PathExists(fs', p)
+//     ensures DirImpliesHasNoAlias(fs', p)
+//     ensures p != RootDir ==> ParentDirIsDir(fs', p)
+//     {
+//       assert |p| > 0;
+//       if p != RootDir {
+//         var parent_dir := GetParentDir(p);
+//         var parent_id := fs.path_map[parent_dir];
+
+//         if p == dst {
+//         } else if InDir(dst, p) {
+//           var srcpath := src + p[|dst|..];
+//           var srcparent_dir := GetParentDir(srcpath);
+//           assert ParentDirIsDir(fs, srcpath);
+//           assert parent_dir == dst || InDir(dst, parent_dir); // observe
+//           assert src + parent_dir[|dst|..] == srcparent_dir; // observe
+//         } else {
+//           assert PathExists(fs, p);
+//           assert ParentDirIsDir(fs, p); // observe
+//           assert fs.path_map[parent_dir] == fs'.path_map[parent_dir];
+//         }
+//         assert ParentDirIsDir(fs', p);
+//       }
+
+//       var id := fs'.path_map[p];
+//       var m := fs'.meta_map[id];
+//       var aliases := AliasPaths(fs', id);
+
+//       if (exists path | path in aliases :: path == dst || InDir(dst, path)) {
+//         // this covers cases for dst prefixes and old src's aliases
+//         if m.ftype.Directory? && !NoAlias(fs', p) {
+//           var path :| path in aliases && (path == dst || InDir(dst, path));
+//           var aliaspath :| aliaspath in aliases && aliaspath != path;
+//           assert path != aliaspath;
+
+//           var srcpath := src + path[|dst|..];
+//           assert id == fs.path_map[srcpath];
+//           assert DirImpliesHasNoAlias(fs, srcpath); // observe
+
+//           if aliaspath == dst || InDir(dst, aliaspath) {
+//             var srcalias := src + aliaspath[|dst|..];
+//             assert fs.path_map[srcalias] == fs'.path_map[aliaspath];
+//             RenamedPathsRemainDifferent(src, dst, path, aliaspath);
+//             assert srcalias != srcpath;
+//             assert false;
+//           } else {
+//             assert fs.path_map[aliaspath] == fs'.path_map[aliaspath]; 
+//             assert false;
+//           }
+//         }
+//       } else {
+//         assert DirImpliesHasNoAlias(fs, p); // observe
+//         assert DirImpliesHasNoAlias(fs', p);
+//       }
+//     }
+  
+//     assert Inv(fs');
+//   }
+
+//   lemma RenamePreservesInv(fs: FileSys, fs': FileSys, source: Path, dest: Path, ctime: Time)
+//   requires Inv(fs)
+//   requires Rename(fs, fs', source, dest, ctime)
+//   ensures Inv(fs')
+//   {
+//     var m := fs.meta_map[fs.path_map[source]];
+//     if m.ftype.Directory? {
+//       RenameDirPreservesInv(fs, fs', source, dest, ctime);
+//     } else {
+//       RenameNonDirPreservesInv(fs, fs', source, dest, ctime);
+//     }
+//   }
+
+//   lemma LinkPreservesInv(fs: FileSys, fs': FileSys, source: Path, dest: Path, ctime: Time)
+//   requires Inv(fs)
+//   requires Link(fs, fs', source, dest, ctime)
+//   ensures Inv(fs')
+//   {
+//     forall p | PathExists(fs', p)
+//     ensures DirImpliesHasNoAlias(fs', p)
+//     ensures p != RootDir ==> ParentDirIsDir(fs', p)
+//     {
+//       assert p != dest ==> DirImpliesHasNoAlias(fs, p); // observe
+//       assert p != RootDir ==> ParentDirIsDir(fs, p); // observe
+
+//       var id := fs.path_map[source];
+//       if fs'.path_map[p] != id {
+//         SameAliases(fs, fs', AliasPaths(fs', id), iset{id});
+//       }
+//     }
+
+//     assert Inv(fs');
+//   }
+
+//   lemma SimpleStepPreservesInv(fs: FileSys, fs': FileSys, step: Step)
+//   requires Inv(fs)
+//   requires NextStep(fs, fs', step)
+//   requires step.CreateStep? || step.SymLinkStep? || step.ChangeAttrStep?
+//         || step.TruncateStep? || step.WriteStep? || step.UpdateTimeStep?
+//   ensures Inv(fs')
+//   {
+//     var path := if step.SymLinkStep? then step.dest else step.path;
+
+//     forall p | PathExists(fs', p)
+//     ensures DirImpliesHasNoAlias(fs', p)
+//     ensures p != RootDir ==> ParentDirIsDir(fs', p)
+//     {
+//       if p != path {
+//         assert PathExists(fs, p); // observe
+//         assert DirImpliesHasNoAlias(fs, p); // observe
+
+//         if step.SymLinkStep? || step.CreateStep? {
+//           SameAliases(fs, fs', iset{path}, iset{fs'.path_map[path]});
+//         }
+//       }
+//     }
+
+//     assert Inv(fs');
+//   }
+}
